src/Init/Prelude.lean
@@ -1954,12 +1954,14 @@ The type of unsigned 16-bit integers. This type has special support in the
 compiler to make it actually 16 bits rather than wrapping a `Nat`.
 -/
 structure UInt16 where
-  /-- Unpack a `UInt16` as a `Nat` less than `2^16`.
+  /-- Unpack a `UInt16` as a `BitVec 16`.
   This function is overridden with a native implementation. -/
-  val : Fin UInt16.size
+  toBitVec : BitVec 16
 
 attribute [extern "lean_uint16_of_nat_mk"] UInt16.mk
-attribute [extern "lean_uint16_to_nat"] UInt16.val
+attribute [extern "lean_uint16_to_nat"] UInt16.toBitVec
+
+def UInt16.val (x : UInt16) : Fin UInt16.size := x.toBitVec.toFin
 
 /--
 Pack a `Nat` less than `2^16` into a `UInt16`.
@@ -1967,7 +1969,7 @@ This function is overridden with a native implementation.
 -/
 @[extern "lean_uint16_of_nat"]
 def UInt16.ofNatCore (n : @& Nat) (h : LT.lt n UInt16.size) : UInt16 where
-  val := { val := n, isLt := h }
+  toBitVec := BitVec.ofNatLt n h
 
 set_option bootstrap.genMatcherCode false in
 /--
@@ -1978,7 +1980,9 @@ This function is overridden with a native implementation.
 def UInt16.decEq (a b : UInt16) : Decidable (Eq a b) :=
   match a, b with
   | ⟨n⟩, ⟨m⟩ =>
-    dite (Eq n m) (fun h => isTrue (h ▸ rfl)) (fun h => isFalse (fun h' => UInt16.noConfusion h' (fun h' => absurd h' h)))
+    dite (Eq n m)
+      (fun h => isTrue (h ▸ rfl))
+      (fun h => isFalse (fun h' => UInt16.noConfusion h' (fun h' => absurd h' h)))
 
 instance : DecidableEq UInt16 := UInt16.decEq
 
